---
{"dg-publish":true,"permalink":"/MATH/抽象代数III/Nodes/7 250408/","dgPassFrontmatter":true}
---


Let $1=e_1+\cdots+e_n$ be a primitive idempotent decomposition in $A/J(A)$. Let $1=f_1+\cdots+f_n$ be a primitive idempotent decomposition in $A$ with $e_i=f_i+J(A)$. 

> [!definition]
> We denote by $c_{ij}$ the multiplicity of $(A/J(A))e_i$ in $Af_j$, which is called the Cartan variant in $A$. The $n\times n$ matrix $(c_{ij})_{n\times n}$ is called the Cartan matrix of $A$. 

> [!theorem]
> $c_{ij}\neq 0$ iff $f_iAf_j\neq 0$. 


For convenience, if $S$ and $T$ are two simple $A$-modules, we denote by $C_{ST}$, the corresponding Cartan invariant, i.e., the multiplicity of $S$ in $P_T$. 


> [!proposition]
> Let $A$ be a finitely generated $k$-algebra over a field $k$, and $S$ a simple $A$-module with projective over $P_S$. 
> Let $A$ be a finitely dimensional $A$-module. 
> - If $T$ is a simple $A$-module, then 
>   
>   $$\dim_k\mathrm{Hom}_A(P_S,T)=\begin{cases}\dim\mathrm{End} _A(S)&\text{if }S\simeq T,\\ 0 &\text{otherwise.}\end{cases}$$
>   
> - The multiplicity of $S$ in $U$ is $\dim\mathrm{Hom}_A(P_S,U)/\dim \mathrm{End}_A(S)$. 
> - If $e\in A$ is an idempotent, then $\dim\mathrm{Hom}(Ae,U)=\dim eU$.
> - Let $e_S$ and $e_T$ be idempotents so that $P_S=Ae_S$ and $P_T=Ae_T$ are projective covers of $S$ and $T$. Then 
>   
>   $$C_{ST}=\dim\mathrm{Hom}_A(P_S,P_T)/\mathrm{End}_A(S)=\dim e_SAe_T/\dim \mathrm{End}_A(S).$$
>   
>   If moreover $k=\overline k$, then $C_{ST}=\dim\mathrm{Hom}_A(P_S,P_T)=\dim e_S Ae_T$. 

**_Proof._**
i) If $P_S\to T$ is nonzero, then the kernel must be a maximal submodule, containing $\mathrm{Rad}(P_S)$. But $P_S/\mathrm{Rad}(P_S)\simeq S$, so $S\simeq T$. Note that there is a commutative diagram

![Pasted image 20250408192218.png|160](/img/user/%E9%99%84%E4%BB%B6/Pasted%20image%2020250408192218.png)

one have $\mathrm{Hom}_A(S,T)\simeq \mathrm{End}_A(S)$. 

ii)- 据说后面都是显然的，我没看啊我没看
<p align="left">□</p>




Let $R$ be a commutative ring with $1$. For $R$-modules $X,Y$ and $M$, we have an $R$-morphism 

$$\begin{aligned}
\mathrm{Hom}_R(X,M)\otimes_R\mathrm{Hom}_R(M,Y)&\to \mathrm{Hom}_R(X,Y),\\
\varphi\otimes \psi&\mapsto \psi\varphi.
\end{aligned}$$

> [!proposition]
> The image of this morphism is comprised of those morphism from $X$ to $Y$ which factor through some finite power of $M$.
> 
> ![Pasted image 20250408192748.png|160](/img/user/%E9%99%84%E4%BB%B6/Pasted%20image%2020250408192748.png)

**_Proof._**
An element of the image is $\sum_{i\in I}\psi_i\varphi_i$, where $\psi_i:X\to M$ and $\varphi_i:M\to Y$. Give a morphism $\varphi:X\to M^I,x\mapsto (\varphi_i(x))$ and a morphism $\psi:M^I\to Y,(m_i)\to \sum \psi_i(m_i)$. Now we finish the proof.
<p align="left">□</p>


Recall that $X^*=\mathrm{Hom}_R(X,R)$ is the dual (?)

Taking $M=R$, we get a morphism $\tau_{X,Y}:X^*\otimes Y\to \mathrm{Hom}_R(X,Y)$. Denote by $\mathrm{Hom}^{\rm pr}_R(X,Y)$ the image of $\tau_{X,Y}$, and the elementary $\mathrm{Hom}_R^{\rm pr}(X,Y)$ are called the projective morphism from $X$ to $Y$. 

> [!lemma]
> For any $R$-module $M$, $\mathrm{Hom}_R^{\rm pr}(M,M)$ is a $2$-sided ideal of the ring $\mathrm{End}_R(M)=\mathrm{Hom}_R(M,M)$. 

**_Proof._**
- [ ] exercise.
<p align="left">□</p>


> [!theorem] 
> Let $P$ be an $R$-module. TFAE:
> - $P$ is a finitely generated projective module.
> - $\mathrm{Hom}_R^{\rm pr}(P,P)=\mathrm{End}_R(P)$.
> - For any $R$-module $X$, the morphism $\tau_{X,P}:X^*\otimes_R P\to \mathrm{Hom}_R(X,P)$ is an isomorphism.
> - For any $R$-module $X$, the morphism $\tau_{P,X}:P^*\otimes X\to\mathrm{Hom}_R(P,X)$ is an isomorphism.
> - The morphism $\tau_{P,P}:P^*\otimes_R P\to \mathrm{End}_R(P)$ is an isomorphism. 

**_Proof._**
i)->ii) Since $P$ is projective, $P$ is a direct summand of $R^n$. Then by the following diagram we finish the proof.

![Pasted image 20250408194639.png|160](/img/user/%E9%99%84%E4%BB%B6/Pasted%20image%2020250408194639.png)

ii)->iii) Assume $\mathrm{id}_P=\tau_{P,P}(\sum_{i\in I}\varphi_i\otimes m_i)$, then $v=\varphi_i(v)m_i$ for any $v\in P$. Consider the morphism 

$$\begin{aligned}
\sigma:\mathrm{Hom}_R(X,P)&\to X^*\otimes P,\\
\alpha&\mapsto \sum_{i\in I} \varphi_i\alpha\otimes m_i
\end{aligned}$$

Check: $\sigma$ is the inverse of $\tau_{X,P}$. 

Note that

$\mathrm{Hom}_R(X,P)\stackrel{\sigma}{\to}X^*\otimes_R P\stackrel{\tau_{X,P}}{\to} \mathrm{Hom}_R(X,P),\alpha\mapsto \sum_i\varphi_i\alpha\otimes m_i\mapsto (x\mapsto \sum_i\varphi_i(\alpha(x))m_i)$

$X^*\otimes P\stackrel{\tau_{X,P}}{\to}\mathrm{Hom}_R(X,P)\stackrel{\sigma}{\to} X^*\otimes_R P$. 

We will check $\psi\otimes v=\sum_i\varphi_i\tau_{X,P}(\psi\otimes v)\otimes m_i$. Observe that $\varphi_i(v)\psi=\varphi_i\cdot \tau_{X,P}(\psi\otimes v)$. 

Hence $\psi\otimes v=\psi\otimes(\sum_i \varphi_i(v)m_i)=\sum_i\psi\otimes\varphi_i(v)m_i=\sum_i\varphi_i(v)\psi\otimes m_i=\sum_i\varphi_i\tau_{X,P}(\psi\otimes v)\otimes m_i$. 

v)->i) $\mathrm{id}_P$ is projective. $\mathrm{id} =gf$. So $P$ is a direct summand of $R^n$. 


![Pasted image 20250408201031.png|160](/img/user/%E9%99%84%E4%BB%B6/Pasted%20image%2020250408201031.png)

<p align="left">□</p>


# Integrality

Let $S$ be an commutative integral domain with $1$.

> [!definition]
> Let $R$ be a subring of $S$ containing $1_S$. We say $\alpha$ is an integral element over $R$, if there exists a monic polynomial $f(x)\in R[x]$ such that $f(\alpha)=0$. 


> [!proposition]
> Let $S,R$ be rings and $\alpha\in S$. TFAE:
> - $\alpha$ is an integral domain over $R$
> - $R[\alpha]$ is a finitely generated $R$-module.
> - There exists a subring $T$ of $S$ with $R\subseteq T$ such that $T$ is a finitely generated $R$-module and $\alpha\in T$. 

**_Proof._**
ii)->iii) Take $T=R[\alpha]$. 

i)->ii) There is $f(x)=x^n+a_{n-1}x^{n-1}+\cdots+a_1x+a_0$ with $f(\alpha)=0$. Then $\alpha^n=-\sum_{i=0}^{n-1}a_i\alpha^i$ is a linear combination of $1,\alpha,\cdots,\alpha^{n-1}$. It deduces that $R[\alpha]$ is generated by $1,\alpha,\cdots,\alpha^{n-1}$. 

iii)->i) Let $\epsilon_1,\cdots,\epsilon_n$ be a generator set of $T$ as an $R$-module. Write $\alpha\epsilon_i=a_{i1}\epsilon_1+\cdots+a_{in}\epsilon_n$ with $a_{ij}\in R$. It deduces that $-a_{i1}\epsilon_1+\cdots+(\alpha-a_{ii})\epsilon_i+\cdots+(-a_{in}\epsilon_n)=0$ and so

$$\begin{pmatrix}\epsilon_1 & \cdots & \epsilon_n\end{pmatrix}\begin{pmatrix}
\alpha-a_{11} & -a_{21} & \cdots & -a_{n1} \\
-a_{12} & \alpha-a_{22} & \cdots & -a_{n2} \\
\vdots & \vdots & \ddots & \vdots \\
-a_{1n} & -a_{2n} & \cdots & \alpha-a_{nn}
\end{pmatrix}=\begin{pmatrix}0 & \cdots & 0\end{pmatrix}$$

where $A=\begin{pmatrix}\alpha-a_{11} & -a_{21} & \cdots & -a_{n1} \\-a_{12} & \alpha-a_{22} & \cdots & -a_{n2} \\\vdots & \vdots & \ddots & \vdots \\-a_{1n} & -a_{2n} & \cdots & \alpha-a_{nn}\end{pmatrix}$. Multiplying $A^*$, we have $(\epsilon_1,\cdots,\epsilon_n)\mathrm{diag}(\det A,\cdots,\det A)=(0,\cdots,0)$. Hence $\epsilon_i\det A=0$ and so $\det A =0$. Therefore, $\alpha$ is integral over $R$. 
<p align="left">□</p>


> [!lemma]
> $S,R$ are as above. $R\subseteq M_i\subseteq S$ where $M_i$ are subrings of $S$. If $M_1,M_2$ are finitely generated $R$-modules, then the ring $R[M_1,M_2]$ is finitely generated as an $R$-module. 

**_Proof._**
- [ ] Exercise.
<p align="left">□</p>

> [!theorem]
> $S,R$ are as above. The integral elements of $S$ over $R$ form a subring of $S$ containing $R$. 

**_Proof._**
$\alpha,\beta$ integral -> $R[\alpha],R[\beta]$ f.g.-> $R[\alpha,\beta]$ f.g. -> $\alpha-\beta$, $\alpha\beta$ integral
<p align="left">□</p>


> [!definition]
> - $R,S$ are as above. The subring of $S$ containing of integral of $S$ over $R$ is called the integral closure of $R$ in $S$. 
> - $R$ is called integral closed in $S$ if every integral elements of $S$ over $R$ is containing in $R$.
> - We say an integral domain $R$ is integral closed if it is integral closed in tis fractional field.
> - $\mathbb{Z}\subseteq \mathbb{C}$, if $z\in \mathbb{C}$ is integral over $\mathbb{Z}$, we call $z$ an algebraic integer. All algebraic integer form a ring. 

> [!theorem]
> A UFD is integral closed. 

**_Proof._**
HW
<p align="left">□</p>


# Torsion and torsion free elements

> [!definition]
> Let $R$ be a ring, and let $M$ be a $R$-module. $m\in M$ is said to be 
> - a torsion element if $\mathrm{Ann}_R(m)\neq 0$
> - a torsion free element if $\mathrm{Ann}_R(m)=0$. 


**Example.** 
- $\mathbb{Z}$-module $\mathbb{Q}$ has no torsion element but $0$. 
- $R$ is commutative,
	- ${}_R R$ has no torsion element but $0$ iff $R$ is an integral domain;
	- if $I$ is a proper ideal, all element if $R$-module $R/I$ are torsion;
	- $R/I$ has no torsion element but $0$, iff $I$ is prime. 

> [!lemma]
> If $R$ is an integral domain, the subset of $M$ 
> 
> $$\mathrm{tor}(M)=\{m\subseteq M:\mathrm{Ann} _R(m)\neq 0\}$$
> 
> is a submodule of $M$, which is called the torsion submodule of $M$. 

> [!definition]
> We say $M$ is a torsion module if $M=\mathrm{tor}(M)$, and $M$ is torsion free if $\mathrm{tor}(M)=0$. 

**Examples.** 
- $\mathbb{Z}$-modules: $\mathbb{Z},\mathbb{Q},\mathbb{Z}/2\mathbb{Z}$, $\mathrm{tor}(\mathbb{Q})=0$ and $\mathrm{tor}(\mathbb{Z}/2\mathbb{Z})=\mathbb{Z}/2\mathbb{Z}$
- For an integral domain $R$ and a $R$-module $M$, $\mathrm{tor}(M^*)=0$ where $M^*=\mathrm{Hom}_R(M,R)$.

> [!proposition]
> Let $R$ be an integral domain. Free modules are torsion free. 

> [!proposition]
> Let $R$ be an integral domain. Any finitely generated torsion free $R$-module is isomorphic to a submodule of a free $R$-module of finite rank.

**_Proof._**
Suppose $M$ is generated by non-zero elements $x_1,\cdots,x_n$. Up to reordering, assume $x_1,\cdots,x_r$ is a maximal linearly independent subset of $x_1,\cdots,x_n$. If $r=n$, then $M$ is free. 

Assume $r<n$. Consider $M_n=Rx_1+\cdots+Rx_r=Rx_1\oplus\cdots\oplus Rx_r$. For each $j\geqslant r+1$, there exists $\lambda_j\in R$ such that $\lambda_jx_j\in M_0$. Let $\lambda=\lambda_{r+1}\cdots\lambda_m$. Then $\lambda M\subseteq M_0$. Consider $M\to M_0,m\mapsto \lambda m$, which is injective. Therefore, $M$ is isomorphic to a free $R$-module of finite rank.
<p align="left">□</p>


# Localization


<div class="transclusion internal-embed is-loaded"><a class="markdown-embed-link" href="/math//nodes/3-rings-and-modules-of-fractions/#d61f0b" aria-label="Open link"><svg xmlns="http://www.w3.org/2000/svg" width="24" height="24" viewBox="0 0 24 24" fill="none" stroke="currentColor" stroke-width="2" stroke-linecap="round" stroke-linejoin="round" class="svg-icon lucide-link"><path d="M10 13a5 5 0 0 0 7.54.54l3-3a5 5 0 0 0-7.07-7.07l-1.72 1.71"></path><path d="M14 11a5 5 0 0 0-7.54-.54l-3 3a5 5 0 0 0 7.07 7.07l1.71-1.71"></path></svg></a><div class="markdown-embed">



> [!proposition]
> There exists unique $S^{-1}A$-module isomorphism 
> 
> $f:S^{-1}A\otimes_A M\simeq S^{-1}M,a/s\otimes m\mapsto am/s.$
> 
> 

</div></div>


Set $FM=F\otimes_R M=S^{-1}M$ with $S=R\setminus \{0\}$. The kernel of $M\to FM,m\mapsto 1\otimes m$ is $\mathrm{tor}(M)$. 

> [!corollary]
> - $F\otimes_R \mathrm{tor}(M)=0$
> - TFAE:
>     - the natural $R$-morphism $M\to FM,m\mapsto 1\otimes m$ is injective
>     - $M$ is torsion free.

> [!corollary]
> If $M$ is finitely generated projective $R$-module, then $M\to FM,m\mapsto 1\otimes m$ is injective. 

> [!definition]
> The rank of a finitely generated torsion free $R$-module is the dimension of the $F$-space $FM$. 

**Remark.** A finitely generated torsion free $R$-module $M$ of rank one is isomorphic to a finitely generated $R$-submodule of $F$. Indeed, if $FM=Fe$, then $I=\{\lambda\in F:\lambda e\in M\}$ is an $R$-submodule of $F$. We have $M=Ie$. 

Let $M$ be a finitely generated torsion free $R$-module. $F\to FM,m\mapsto 1\otimes m$ injective. So $M$ can be viewed as an $R$-submodule of $FM$. Given an $F$-basis $(e_i)_{1\leqslant i\leqslant r}$ of $FM$, assume $M$ is generated by $m_1,\cdots,m_n$. Then 

$$m_i=\frac{s_1}{t_1}e_1+\cdots+\frac{s_r}{t_r}e_r$$

with $s_i\in R$ and $t_i\in R\setminus \{0\}$. There exists $\lambda\in R\setminus\{0\}$ such that $\lambda M\subseteq Re_1\oplus\cdots\oplus R e_r$. Additionally, $M$ generated $FM$. 

> [!definition]
> Let $V$ be an $F$-vector space of finitely generated $r$. A fractional $R$-module in $V$ is an $R$-submodule of $V$ such that
> - $M$ generates $V$;
> - given any basis $(e_i)_{1\leqslant i\leqslant r}$ of $V$, there exists $\lambda\in R$ with $\lambda\neq 0$ such that $\lambda M\subseteq \oplus_{i=1}^r Re_i$. 

In the case $V=F$, fractional modules are called fractional ideals of $R$. It is an $R$-submodule $I$ of $F$ such that there exists nonzero $\lambda\in R$ such that $\lambda I\subseteq R$. Hence $\lambda I$ is an ideal of $R$. 
- every finitely generated $R$-submodule of $F$ is a fractional ideal
- if $R$ is Noetherian, then these are all fractional ideals. That is, when $R$ is Noetherian, finitely generated $R$-module $\iff$ fractional ideal.

> [!check] the proof of the second statement
> Let $R$ be a Noetherian integral domain and $F = \mathrm{Frac}(R)$. Let $I$ be an $R$-submodule of $F$. We want to show that $I$ is a fractional ideal if and only if $I$ is finitely generated.
> 
> ($\implies$) Assume $I$ is finitely generated. Let $I = \sum_{k=1}^n R x_k$ for some $x_k \in I$. Since $x_k \in F$, we can write $x_k = p_k / q_k$ where $p_k, q_k \in R$ and $q_k \neq 0$. Let $\lambda = q_1 q_2 \dots q_n$. Then $\lambda \in R$ and $\lambda \neq 0$. For each $k$, $\lambda x_k = (q_1 \dots q_{k-1} q_{k+1} \dots q_n) p_k \in R$. Then $\lambda I = \sum_{k=1}^n R (\lambda x_k) \subseteq R$. By definition, $I$ is a fractional ideal.
> 
> ($\impliedby$) Assume $I$ is a fractional ideal. By definition, $I$ is an $R$-submodule of $F$ and there exists $\lambda \in R \setminus \{0\}$ such that $\lambda I \subseteq R$. Let $J = \lambda I$. Note that $J$ is an $R$-submodule of $R$, which means $J$ is an ideal of $R$. Since $R$ is a Noetherian ring, the ideal $J$ must be finitely generated. Let $J = \sum_{k=1}^n R y_k$ for some $y_k \in J$. Since $y_k \in J = \lambda I$, we can write $y_k = \lambda x_k$ for some $x_k \in I$. We claim $I = \sum_{k=1}^n R x_k$.
> 
> Take any $x \in I$. Then $\lambda x \in J$. So, $\lambda x = \sum_{i=1}^n r_i y_i$ for some $r_i \in R$. Substituting $y_i = \lambda x_i$, we get $\lambda x = \sum_{i=1}^n r_i (\lambda x_i) = \lambda (\sum_{i=1}^n r_i x_i)$. Since $\lambda \neq 0$ and $F$ is a field, we can multiply by $1/\lambda$ to get $x = \sum_{i=1}^n r_i x_i$. This shows $I \subseteq \sum_{k=1}^n R x_k$. The inclusion $\sum_{k=1}^n R x_k \subseteq I$ is clear since each $x_k \in I$ and $I$ is an $R$-module. Thus, $I = \sum_{k=1}^n R x_k$, which means $I$ is finitely generated.
> 

